Layered specification: kvs user map is always passed around

theories/case_studies/multiuser_kvs/kvs_preamble.v
@@ -376,6 +376,196 @@ Section KVS_physical_map.
     apply elem_of_kvs_keys; eexists _,_; eauto.
   Qed.
 
+  Lemma NoDup_kvs_keys_update (m : kvs_physical_map) (idx : nat) (k : Z) (w w' : Word) :
+    m !! idx = Some (Some (k, w)) ->
+    NoDup (kvs_keys m) ->
+    NoDup (kvs_keys (<[idx := Some (k, w') ]>m)).
+  Proof.
+    move: idx k w w'.
+    induction m using map_ind; intros idx k w w' Hk Hnodup; first simplify_map_eq.
+    destruct (decide (idx = i)); simplify_map_eq.
+    - rewrite insert_insert_eq.
+      rewrite kvs_keys_insert_Some; auto.
+      rewrite kvs_keys_insert_Some in Hnodup; auto.
+    - rewrite insert_insert_ne; last done.
+      destruct x as [ [k' w''] |].
+      + rewrite kvs_keys_insert_Some in Hnodup; auto.
+        rewrite kvs_keys_insert_Some; simplify_map_eq; auto.
+        apply NoDup_cons in Hnodup as [HkX Hnodup].
+        apply NoDup_cons; split; last (eapply IHm; eauto).
+        intro Hcontra.
+        apply elem_of_kvs_keys in Hcontra as (w0 & idx0 & H0).
+        apply HkX.
+        apply elem_of_kvs_keys; auto.
+        destruct (decide (idx = idx0)); simplify_map_eq.
+        { exists w, idx0; done. }
+        { exists w0, idx0; done. }
+      + rewrite kvs_keys_insert_None in Hnodup; auto.
+        rewrite kvs_keys_insert_None; simplify_map_eq; auto.
+        eapply IHm; eauto.
+  Qed.
+
+  Lemma wf_kvs_physical_map_update (m : kvs_physical_map) (idx : nat) (k : Z) (w : Word) :
+    (∃ w', m !! idx = Some (Some (k, w'))) ->
+    wf_kvs_physical_map m ->
+    wf_kvs_physical_map (<[idx:= Some (k, w)]> m).
+  Proof.
+    intros [w' Hidx] (Hkvs_dom & Hkvs_unique).
+    split.
+    - rewrite dom_insert_L -Hkvs_dom.
+      assert (idx ∈ dom m).
+      { apply elem_of_dom; eauto. }
+      set_solver.
+    - eapply NoDup_kvs_keys_update; eauto.
+  Qed.
+
+  Lemma kvs_physical_map_close_update
+    (a : Addr) (pkvs : kvs_physical_map) (idx : nat) (k : full_key_t) (w : Word):
+    (∃ w' : Word, pkvs !! idx = Some (Some (k, w'))) ->
+
+    is_physical_kvs_open a pkvs idx -∗
+    physical_kvs_entry a idx (Some (k,w)) -∗
+    is_physical_kvs a (<[idx:= Some (k,w)]> pkvs).
+  Proof.
+    iIntros (Hidx) "[%Hwf_kvs HKVS] Hentry"; cbn.
+    iDestruct (big_sepM_insert_delete with "[$HKVS $Hentry]") as "HKVS"; eauto.
+    iFrame; eauto.
+    iPureIntro.
+    eapply wf_kvs_physical_map_update; eauto.
+  Qed.
+
+  Lemma NoDup_kvs_keys_insert_Some
+    (m : kvs_physical_map) (idx : nat) (k : Z) (w : Word) :
+    k ∉ kvs_keys m ->
+    NoDup (kvs_keys m) ->
+    NoDup (kvs_keys (<[idx:= Some (k, w)]> m)).
+  Proof.
+    move: idx k w.
+    induction m using map_ind; intros idx k w Hk Hnodup.
+    { rewrite kvs_keys_insert_Some; simplify_map_eq; auto.
+      rewrite kvs_keys_empty.
+      apply NoDup_singleton.
+    }
+    destruct (decide (idx = i)); simplify_map_eq.
+    - rewrite insert_insert_eq.
+      rewrite kvs_keys_insert_Some; auto.
+      destruct x as [ [k' w''] |].
+      + rewrite kvs_keys_insert_Some in Hnodup; auto.
+        rewrite kvs_keys_insert_Some in Hk; auto.
+        apply not_elem_of_cons in Hk as [Hkk' Hk].
+        apply NoDup_cons in Hnodup as [Hk' Hnodup].
+        apply NoDup_cons; split; auto.
+      + rewrite kvs_keys_insert_None in Hnodup; auto.
+        rewrite kvs_keys_insert_None in Hk; auto.
+        apply NoDup_cons; split; auto.
+    - rewrite insert_insert_ne; last done.
+      destruct x as [ [k' w''] |].
+      + rewrite kvs_keys_insert_Some in Hnodup; auto.
+        rewrite kvs_keys_insert_Some in Hk; auto.
+        rewrite kvs_keys_insert_Some; simplify_map_eq; auto.
+        apply not_elem_of_cons in Hk as [Hkk' Hk].
+        apply NoDup_cons in Hnodup as [Hk' Hnodup].
+        apply NoDup_cons; split; auto.
+        intro Hcontra.
+        apply elem_of_kvs_keys in Hcontra.
+        destruct Hcontra as (w0&idx0&Hcontra).
+        destruct (decide (idx0 = idx)); simplify_map_eq.
+        apply Hk'.
+        apply elem_of_kvs_keys.
+        eexists _,_;eauto.
+      + rewrite kvs_keys_insert_None in Hnodup; auto.
+        rewrite kvs_keys_insert_None in Hk; auto.
+        rewrite kvs_keys_insert_None; simplify_map_eq; auto.
+  Qed.
+
+  Lemma wf_kvs_physical_map_insert (m : kvs_physical_map) (idx : nat) (k : Z) (w : Word) :
+    m !! idx = Some None ->
+    k ∉ kvs_keys m ->
+    wf_kvs_physical_map m ->
+    wf_kvs_physical_map (<[idx:= Some (k, w)]> m).
+  Proof.
+    intros Hidx Hk (Hkvs_dom & Hkvs_unique).
+    split.
+    - rewrite dom_insert_L -Hkvs_dom.
+      assert (idx ∈ dom m).
+      { apply elem_of_dom; eauto. }
+      set_solver.
+    - eapply NoDup_kvs_keys_insert_Some; eauto.
+  Qed.
+
+  Lemma kvs_physical_map_close_insert
+    (a : Addr) (pkvs : kvs_physical_map) (idx : nat) (k : full_key_t) (w : Word):
+    pkvs !! idx = Some None ->
+    k ∉ kvs_keys pkvs ->
+
+    is_physical_kvs_open a pkvs idx -∗
+    physical_kvs_entry a idx (Some (k,w)) -∗
+    is_physical_kvs a (<[idx:= Some (k,w)]> pkvs).
+  Proof.
+    iIntros (Hidx Hk) "[%Hwf_kvs HKVS] Hentry"; cbn.
+    iDestruct (big_sepM_insert_delete with "[$HKVS $Hentry]") as "HKVS"; eauto.
+    iFrame; eauto.
+    iPureIntro.
+    eapply wf_kvs_physical_map_insert; eauto.
+  Qed.
+
+  Lemma NoDup_kvs_keys_delete
+    (m : kvs_physical_map) (idx : nat)  :
+    NoDup (kvs_keys m) ->
+    NoDup (kvs_keys (<[idx:=None]> m)).
+  Proof.
+    generalize dependent idx.
+    induction m using map_ind; intros idx Hnodup; first simplify_map_eq.
+    { rewrite kvs_keys_insert_None; auto. }
+    destruct (decide (idx = i)); simplify_map_eq.
+    - rewrite insert_insert_eq.
+      rewrite kvs_keys_insert_None; auto.
+      destruct x as [ [] |].
+      + rewrite kvs_keys_insert_Some in Hnodup; auto.
+        apply NoDup_cons in Hnodup as [ _ Hnodup ]; auto.
+      + rewrite kvs_keys_insert_None in Hnodup; auto.
+    - rewrite insert_insert_ne; auto.
+      destruct x as [ [ k' w' ] |].
+      + rewrite kvs_keys_insert_Some in Hnodup; auto.
+        apply NoDup_cons in Hnodup as [ Hk' Hnodup ]; auto.
+        rewrite kvs_keys_insert_Some; simplify_map_eq; auto.
+        apply NoDup_cons; split ; auto.
+        intro Hk. apply elem_of_kvs_keys in Hk as (?&idx_k&?); simplify_eq.
+        destruct (decide (idx_k = idx)); simplify_map_eq.
+        apply Hk'.
+        apply elem_of_kvs_keys; eexists _,_ ; eauto.
+      + rewrite kvs_keys_insert_None in Hnodup; auto.
+        rewrite kvs_keys_insert_None; simplify_map_eq; auto.
+  Qed.
+
+  Lemma wf_kvs_physical_map_delete (pkvs : kvs_physical_map) (idx : nat) :
+    (is_Some (pkvs !! idx)) ->
+    wf_kvs_physical_map pkvs ->
+    wf_kvs_physical_map (<[idx:=None]> pkvs).
+  Proof.
+    intros [w' Hidx] (Hkvs_dom & Hkvs_unique).
+    split.
+    - rewrite dom_insert_L -Hkvs_dom.
+      assert (idx ∈ dom pkvs).
+      { apply elem_of_dom; eauto. }
+      set_solver.
+    - eapply NoDup_kvs_keys_delete; eauto.
+  Qed.
+
+  Lemma kvs_physical_map_close_delete
+    (a : Addr) (pkvs : kvs_physical_map) (idx : nat) :
+    is_Some (pkvs !! idx) ->
+
+    is_physical_kvs_open a pkvs idx -∗
+    physical_kvs_entry a idx None -∗
+    is_physical_kvs a (<[idx:= None ]> pkvs).
+  Proof.
+    iIntros (Hidx) "[%Hwf_kvs HKVS] Hentry"; cbn.
+    iDestruct (big_sepM_insert_delete with "[$HKVS $Hentry]") as "HKVS"; eauto.
+    iFrame; eauto.
+    iPureIntro.
+    eapply wf_kvs_physical_map_delete; eauto.
+  Qed.
 
 End KVS_physical_map.
 
@@ -487,57 +677,339 @@ Section KVS_logical_map.
     apply Hsync in Hcontra as (m'&Hm'&Hcontra); simplify_map_eq.
   Qed.
 
+
+  Definition kvs_logical_kvs_insert
+    (lkvs : kvs_logical_map) (uk : user_key_t) (mk : map_key_t) (w : Word) :=
+   <[uk := (<[ mk := w ]> (default ∅ (lkvs !! uk))) ]> lkvs.
+
+  Notation "<<[ ( uk , mk ) := w ]>> lkvs" :=
+    (kvs_logical_kvs_insert lkvs uk mk w) (at level 10).
+
+  Lemma kvs_logical_kvs_insert_lookup_eq
+    (lkvs : kvs_logical_map) (uk : user_key_t) (mk : map_key_t) (w : Word) (m : kvs_user_map) :
+    (<<[ ( uk, mk ) := w ]>> lkvs) !! uk = Some m ->
+    m = <[mk := w]> (default ∅ (lkvs !! uk)).
+  Proof.
+    intros H.
+    rewrite /kvs_logical_kvs_insert in H; simplify_map_eq.
+    done.
+  Qed.
+
+  Lemma kvs_logical_kvs_insert_lookup_ne
+    (lkvs : kvs_logical_map) (uk uk' : user_key_t) (mk : map_key_t) (w : Word) (m : kvs_user_map) :
+    uk ≠ uk' ->
+    (<<[ ( uk, mk ) := w ]>> lkvs) !! uk' = Some m ->
+    lkvs !! uk' = Some m.
+  Proof.
+    intros Hk H.
+    rewrite /kvs_logical_kvs_insert in H; simplify_map_eq.
+    done.
+  Qed.
+
+  Lemma NoDup_kvs_keys_elem_of m idx uk mk w idx' uk' mk' w' :
+    let f := kvs_full_key uk mk in
+    let f' := kvs_full_key uk' mk' in
+    NoDup (kvs_keys m) ->
+    idx ≠ idx' ->
+    m !! idx = Some (Some (f, w)) ->
+    m !! idx' = Some (Some (f', w')) ->
+    uk' ≠ uk ∨ mk' ≠ mk.
+  Proof.
+    intros f f'.
+    induction m using map_ind; intros Hnodup Hidx_ne Hm_idx Hm_idx'; first set_solver.
+    simplify_map_eq.
+    destruct x as [ [kx wx] |]; cycle 1.
+    - rewrite kvs_keys_insert_None in Hnodup; auto.
+      assert (idx ≠ i) as Hidx_i_ne by (intro; simplify_map_eq; done).
+      assert (idx' ≠ i) as Hidx'_i_ne by (intro; simplify_map_eq; done).
+      simplify_map_eq.
+      auto.
+    - rewrite kvs_keys_insert_Some in Hnodup; auto.
+      apply NoDup_cons in Hnodup as [Hkx_not_elem_kvs_keys Hnodup].
+      destruct (decide (idx = i)); simplify_map_eq.
+      + (* idx = i *)
+        assert (f' ∈ kvs_keys m) as Hf'.
+        { apply elem_of_kvs_keys; eexists _,_; eauto. }
+        destruct (decide (uk' = uk)); simplify_eq; [right|left]; auto.
+        destruct (decide (mk' = mk)); simplify_eq; auto.
+      + destruct (decide (idx' = i)); simplify_map_eq.
+        * (* idx ≠ i ∧ idx' = i *)
+          assert (f ∈ kvs_keys m) as Hf.
+          { apply elem_of_kvs_keys; eexists _,_; eauto. }
+          destruct (decide (uk' = uk)); simplify_eq; [right|left]; auto.
+          destruct (decide (mk' = mk)); simplify_eq; auto.
+        * (* idx ≠ i ∧ idx' ≠ i *)
+          eapply IHm; eauto.
+  Qed.
+
+  Lemma kvs_synced_logical_kvs_update
+    (m : kvs_physical_map) (lm : kvs_logical_map) (idx : nat) (uk mk : Z) (w : Word) :
+    let k := kvs_full_key uk mk in
+    NoDup (kvs_keys m) ->
+    is_uint16 mk ->
+    (∃ w', m !! idx = Some ( Some (k, w'))) ->
+    kvs_synced_logical_kvs m lm ->
+    kvs_synced_logical_kvs (<[idx:= Some (k, w)]> m) (kvs_logical_kvs_insert lm uk mk w).
+  Proof.
+    intros k.
+    intros Hnodup Hwf [w' Hidx] Halloc [ku kn] w'' Hwf'.
+    specialize (Halloc (ku, kn) w'' Hwf'); cbn in *.
+    split; intros Hk.
+    - rewrite /kvs_elem_of_logical_kvs in Hk.
+      destruct Hk as (umap & Hlm & Hkn).
+      destruct (decide (ku = uk)); simplify_map_eq.
+      + apply kvs_logical_kvs_insert_lookup_eq in Hlm; simplify_eq.
+        destruct (decide (kn = mk)); simplify_map_eq.
+        * eexists idx; simplify_map_eq; done.
+        * assert ( kvs_elem_of_kvs m (kvs_full_key uk kn) w'' ) as (idx'&?).
+          { apply Halloc. eexists;split;eauto.
+            destruct (lm !! uk) eqn:Hlm; rewrite Hlm in Hkn; cbn in * ; simplify_eq.
+            rewrite Hlm.
+            set_solver.
+          }
+          eexists idx'.
+          destruct (decide (idx = idx')); simplify_map_eq; cbn in *.
+          ** rewrite Hidx in H; simplify_map_eq.
+             apply kvs_full_key_inj in H as [? ?]; eauto; simplify_eq.
+          ** by simplify_map_eq.
+      + apply kvs_logical_kvs_insert_lookup_ne in Hlm; simplify_eq; auto.
+        assert ( kvs_elem_of_logical_kvs lm ku kn w'') as Hk'.
+        { eexists ; split; eauto. }
+        eapply Halloc in Hk' as (idx' & Hk).
+        destruct (decide (idx = idx')); simplify_map_eq; cbn in *.
+        ** rewrite Hidx in Hk; simplify_map_eq.
+           apply kvs_full_key_inj in Hk as [? ?]; eauto; simplify_eq.
+        ** by eexists idx'; simplify_map_eq.
+    - destruct Hk as (idx' & Hk).
+      destruct (decide (idx = idx')); simplify_map_eq; cbn in *.
+      + apply kvs_full_key_inj in Hk as [? ?]; eauto; simplify_eq.
+        rewrite /kvs_elem_of_logical_kvs /kvs_logical_kvs_insert.
+        destruct (lm !! ku) as [umap|] eqn:Humap ; simplify_map_eq.
+        * by eexists; split; eauto; simplify_map_eq.
+        * by eexists; split; eauto; simplify_map_eq.
+      + assert ( kvs_elem_of_logical_kvs lm ku kn w'' ) as (umap&Hlm&Hkn).
+        { apply Halloc; eexists; eauto. }
+        rewrite /kvs_elem_of_logical_kvs /kvs_logical_kvs_insert.
+        destruct (decide (uk = ku)); simplify_map_eq; cycle 1.
+        * eexists; split; eauto.
+        * destruct (decide (kn = mk)); simplify_map_eq.
+          ** eexists; split; eauto.
+             subst k.
+             eapply (NoDup_kvs_keys_elem_of m idx ku mk _ idx' ku mk) in Hnodup; eauto.
+             destruct Hnodup as [|]; done.
+          ** by eexists; split; eauto; simplify_map_eq.
+  Qed.
+
+  Local Lemma kvs_synced_logical_kvs_insert_1
+    (m : kvs_physical_map) ( lm : kvs_logical_map )
+    (idx : nat)
+    (uk mk uk' mk' : Z) (w w' : Word) :
+    let fkey := kvs_full_key uk mk in
+    is_uint16 mk ->
+    m !! idx = Some None ->
+    kvs_synced_logical_kvs m lm ->
+    is_uint16 mk' ->
+    kvs_elem_of_logical_kvs (kvs_logical_kvs_insert lm uk mk w) uk' mk' w' ->
+    kvs_elem_of_kvs (<[idx:= Some (fkey, w)]> m) (kvs_full_key uk' mk') w'.
+  Proof.
+    intros fkey Hwf_full_key Hidx Halloc Hwf_full_key' Hk.
+    destruct Hk as (umap & Huk' & Hmk').
+    destruct (decide (uk = uk')); simplify_map_eq.
+    - apply kvs_logical_kvs_insert_lookup_eq in Huk'; simplify_map_eq.
+      destruct (decide (mk' = mk)) as [Hmk_eq | Hmk_eq]; simplify_map_eq.
+      + eexists idx; simplify_map_eq; done.
+      + specialize (Halloc (uk', mk') w' Hwf_full_key'); cbn in *.
+        rewrite /kvs_elem_of_logical_kvs in Halloc.
+        destruct ( lm !! uk' ) as [umap_uk|] eqn:Hlm; rewrite Hlm in Hmk'; last set_solver+Hmk'.
+        cbn in Hmk'.
+        rewrite Hlm in Halloc.
+        assert (∃ umap : kvs_user_map, Some umap_uk = Some umap
+                                       ∧ umap !! mk' = Some w') as IH.
+        { exists umap_uk; split; auto. }
+        apply Halloc in IH.
+        destruct IH as (idx' & Hk).
+        destruct (decide (idx = idx')); simplify_map_eq; cbn in *; auto.
+        by eexists idx'; simplify_map_eq.
+    - apply kvs_logical_kvs_insert_lookup_ne in Huk'; auto; simplify_map_eq.
+      assert (∃ umap : kvs_user_map, lm !! uk' = Some umap ∧ umap !! mk' = Some w') as IH.
+      { exists umap; split; auto. }
+      specialize (Halloc (uk', mk') w' Hwf_full_key'); cbn in *.
+      rewrite /kvs_elem_of_logical_kvs in Halloc.
+      apply Halloc in IH.
+      destruct IH as (idx' & Hk).
+      destruct (decide (idx = idx')); simplify_map_eq; cbn in *; auto.
+      by eexists idx'; simplify_map_eq.
+  Qed.
+
+  Local Lemma kvs_synced_logical_kvs_insert_2
+    (m : kvs_physical_map) ( lm : kvs_logical_map )
+    (idx : nat)
+    (uk mk uk' mk' : Z) (w w' : Word) :
+    let fkey := kvs_full_key uk mk in
+    is_uint16 mk ->
+    m !! idx = Some None ->
+    fkey ∉ kvs_keys m ->
+    kvs_synced_logical_kvs m lm ->
+    is_uint16 mk' ->
+    kvs_elem_of_kvs (<[idx:= Some (fkey, w)]> m) (kvs_full_key uk' mk') w' ->
+    kvs_elem_of_logical_kvs (kvs_logical_kvs_insert lm uk mk w) uk' mk' w'.
+  Proof.
+    intros fkey Hwf_full_key Hidx Hkfree Halloc Hwf_full_key' Hk.
+    specialize (Halloc (uk', mk') w' Hwf_full_key') as IH.
+    destruct Hk as (idx' & Hk).
+    destruct (decide (idx = idx')); simplify_map_eq; cbn in *; auto.
+    - apply kvs_full_key_inj in Hk as [ -> -> ]; eauto.
+      rewrite /kvs_logical_kvs_insert;simplify_map_eq.
+      rewrite /kvs_elem_of_logical_kvs;simplify_map_eq.
+      exists (<[mk':=w']> (default ∅ (lm !! uk'))); split; auto.
+      by simplify_map_eq.
+    - rewrite /kvs_logical_kvs_insert;simplify_map_eq.
+      rewrite /kvs_elem_of_logical_kvs;simplify_map_eq.
+      assert ( kvs_elem_of_kvs m (kvs_full_key uk' mk') w' ) as IHm.
+      { eexists; eauto. }
+      destruct (decide (uk = uk')); simplify_map_eq.
+      + destruct (decide (mk = mk')); simplify_map_eq.
+        * apply (iffLRn (elem_of_kvs_keys m fkey)) in Hkfree.
+          exfalso; apply Hkfree; eexists _,_; eauto.
+        * apply IH in IHm as (umap & Humap & Humap').
+          by eexists ; split; eauto; simplify_map_eq.
+      + apply IH in IHm as (umap & Humap & Humap').
+        eexists ; split; eauto.
+  Qed.
+
+  Lemma kvs_synced_logical_kvs_insert (m : kvs_physical_map) ( lm : kvs_logical_map ) (idx : nat) (uk mk : Z) (w : Word) :
+    let fkey := kvs_full_key uk mk in
+    is_uint16 mk ->
+    m !! idx = Some None ->
+    fkey ∉ kvs_keys m ->
+    kvs_synced_logical_kvs m lm ->
+    kvs_synced_logical_kvs (<[idx:=Some (fkey, w)]> m) ( kvs_logical_kvs_insert lm uk mk w).
+  Proof.
+    intros fkey Hwf_full_key Hidx Hk_free Halloc.
+    intros [uk' mk'] Hwf_full_key'.
+    cbn.
+    split; intros Hk.
+    - eapply kvs_synced_logical_kvs_insert_1; eauto.
+    - eapply kvs_synced_logical_kvs_insert_2; eauto.
+  Qed.
+
+
+  Definition kvs_logical_kvs_delete (lm : kvs_logical_map) (uk : user_key_t) (mk : map_key_t) :=
+   <[uk := (delete mk (default ∅ (lm !! uk))) ]> lm.
+
+  Notation "lkvs <∖> ( uk , mk )" :=
+    (kvs_logical_kvs_delete lkvs uk mk) (at level 10).
+
+  Lemma kvs_logical_kvs_delete_lookup_eq
+    (lkvs : kvs_logical_map) (uk : user_key_t) (mk : map_key_t) (m : kvs_user_map) :
+    (lkvs <∖> (uk, mk)) !! uk = Some m ->
+    m = delete mk (default ∅ (lkvs !! uk)).
+  Proof.
+    intros H.
+    rewrite /kvs_logical_kvs_delete in H; simplify_map_eq.
+    done.
+  Qed.
+
+  Lemma kvs_logical_kvs_delete_lookup_ne
+    (lkvs : kvs_logical_map) (uk uk' : user_key_t) (mk : map_key_t) (m : kvs_user_map) :
+    uk ≠ uk' ->
+    (lkvs <∖> (uk, mk)) !! uk' = Some m ->
+    lkvs !! uk' = Some m.
+  Proof.
+    intros Hk H.
+    rewrite /kvs_logical_kvs_delete in H; simplify_map_eq.
+    done.
+  Qed.
+
+  Local Lemma kvs_synced_logical_kvs_delete_1
+    (m : kvs_physical_map) (lm : kvs_logical_map) (idx : nat) (uk mk uk' mk' : Z) (w w' : Word) :
+    let fkey := kvs_full_key uk mk in
+    is_uint16 mk ->
+    m !! idx = Some (Some (fkey, w)) ->
+    kvs_synced_logical_kvs m lm ->
+    is_uint16 mk' ->
+    kvs_elem_of_logical_kvs (kvs_logical_kvs_delete lm uk mk) uk' mk' w' ->
+    kvs_elem_of_kvs (<[idx:= None]> m) (kvs_full_key uk' mk') w'.
+  Proof.
+    intros fkey Hwf_full_key Hidx Halloc Hwf_full_key' Hk.
+    destruct Hk as (umap & Huk' & Hmk').
+    destruct (decide (uk = uk')); simplify_map_eq.
+    - apply kvs_logical_kvs_delete_lookup_eq in Huk'; simplify_map_eq.
+      assert ( mk ≠ mk' ) as Hmk_eq ; simplify_map_eq.
+      { intro; simplify_map_eq. }
+        destruct ( lm !! uk' ) as [umap_uk|] eqn:Hlm; rewrite Hlm in Hmk' ; last set_solver+Hmk'.
+      cbn in *.
+      assert ( kvs_elem_of_logical_kvs lm uk' mk' w') as Helem.
+      { eexists; split;eauto. }
+      specialize (Halloc (uk', mk') w' Hwf_full_key'); cbn in *.
+      apply Halloc in Helem as (idx'&Hidx').
+      eexists idx'.
+      destruct (decide (idx = idx')); simplify_map_eq; cbn in *; auto.
+      rewrite Hidx in Hidx'; simplify_map_eq.
+      apply kvs_full_key_inj in Hidx' as [_ ->]; eauto; done.
+    - apply kvs_logical_kvs_delete_lookup_ne in Huk'; auto; simplify_map_eq.
+      assert (∃ umap : kvs_user_map, lm !! uk' = Some umap ∧ umap !! mk' = Some w') as IH.
+      { exists umap; split; auto. }
+      apply (Halloc (uk', mk') w' Hwf_full_key') in IH as (idx'&Hidx').
+      destruct (decide (idx = idx')); simplify_map_eq; cbn in *; auto.
+      * rewrite Hidx in Hidx'; simplify_map_eq.
+        apply kvs_full_key_inj in Hidx' as [-> ->] ;eauto; done.
+      * by exists idx'; simplify_map_eq.
+  Qed.
+
+  Local Lemma kvs_synced_logical_kvs_delete_2
+    (m : kvs_physical_map) (lm : kvs_logical_map) (idx : nat) (uk mk uk' mk' : Z) (w w' : Word) :
+    let fkey := kvs_full_key uk mk in
+    is_uint16 mk ->
+    m !! idx = Some (Some (fkey, w)) ->
+    NoDup (kvs_keys m) ->
+    kvs_synced_logical_kvs m lm ->
+    is_uint16 mk' ->
+    kvs_elem_of_kvs (<[idx:= None]> m) (kvs_full_key uk' mk') w' ->
+    kvs_elem_of_logical_kvs (kvs_logical_kvs_delete lm uk mk) uk' mk' w'.
+  Proof.
+    intros fkey Hwf_full_key Hidx Hnodup Halloc Hwf_full_key' Hk.
+    specialize (Halloc (uk', mk') w' Hwf_full_key') as IH'.
+    cbn in *.
+    destruct Hk as (idx' & Hk).
+
+    destruct (decide (idx = idx')); simplify_map_eq; cbn in *; auto.
+    assert (kvs_elem_of_kvs m (kvs_full_key uk' mk') w') as IHm'.
+    { eexists; eauto. }
+
+    apply IH' in IHm' as (umap' & Humap' & Hmk'_in_umap').
+    assert (kvs_full_key uk mk ∈ kvs_keys m) as IHm.
+    { apply elem_of_kvs_keys; eexists _,_; eauto. }
+    rewrite /kvs_logical_kvs_delete.
+    destruct (decide (uk = uk')); simplify_map_eq; cycle 1.
+    { exists umap'; split; simplify_map_eq;eauto. }
+    eexists (delete mk umap'); split; simplify_map_eq; eauto.
+    destruct (decide (mk = mk')); simplify_map_eq; try done.
+
+    eapply (NoDup_kvs_keys_elem_of m idx uk' mk' _ idx' uk' mk') in Hnodup; eauto.
+    destruct Hnodup as [ | ]; done.
+  Qed.
+
+  Lemma kvs_synced_logical_kvs_delete (m : kvs_physical_map) (lm : kvs_logical_map) (idx : nat) (uk mk : Z) (w : Word) :
+    let fkey := kvs_full_key uk mk in
+    NoDup (kvs_keys m) ->
+    is_uint16 mk ->
+    m !! idx = Some (Some (fkey, w)) ->
+    kvs_synced_logical_kvs m lm ->
+    kvs_synced_logical_kvs (<[idx:=None]> m) (kvs_logical_kvs_delete lm uk mk).
+  Proof.
+    intros fkey Hnodup Hwf_full_key Hidx Halloc.
+    intros [uk' mk'] Hwf_full_key'.
+    cbn.
+    split; intros Hk.
+    - eapply (kvs_synced_logical_kvs_delete_1 m lm idx uk mk uk' mk'); eauto.
+    - eapply (kvs_synced_logical_kvs_delete_2 m lm idx uk mk uk' mk'); eauto.
+  Qed.
+
+
 End KVS_logical_map.
 
 
-(* Section KVS_user_map. *)
-(*   Context *)
-(*     {Σ:gFunctors} *)
-(*     {ceriseg:ceriseG Σ} *)
-(*     {kvsg:kvsG Σ} *)
-(*     `{MP: MachineParameters} *)
-(*   . *)
-
-(*   Definition is_user_kvs `{kvs_namespaces} (a : Addr) (uk : user_key_t) (m : kvs_user_map) : iProp Σ := *)
-(*     logical_kvs_inv a ∗ uk ↦(LKVS) m. *)
-
-(*   Definition kvs_user_pointsto (uk : user_key_t) (mk : map_key_t) (w : Word) := *)
-(*     (uk,mk) ↦(UKVS) w *)
-
-
-
-
-(* End KVS_user_map. *)
-
-(*     ●(KVS) m ∗ *)
-(*     ↪●KVS_USERS lm ∗ *)
-
-
-
-
-
-
-
-
-(* Definition kvs_frag_idx_frac `{kvsG} (idx : nat) (k : Z) (w : Word) (q : dfrac) : iProp Σ := *)
-(*   (pointsto (L:=nat) (V:=kvs_entry) idx q (Some (k,w))). *)
-(* Notation "k '⤇(KVS){' q '}[' idx  ']' w" := *)
-(*   (kvs_frag_idx_frac idx k w q) (at level 20) : bi_scope. *)
-(* Notation "k '⤇(KVS){' q '}[' idx  ']' -" := *)
-(*   (∃ w, kvs_frag_idx_frac idx k w q)%I (at level 20) : bi_scope. *)
-
-(* Notation "idx '⤇(KVS)' 'NONE'" := *)
-(*   (pointsto (L:=nat) (V:=kvs_entry) idx (DfracOwn 1) None) (at level 20) : bi_scope. *)
-(* Notation "k '⤇(KVS)[' idx  ']' w" := *)
-(*   (kvs_frag_idx_frac idx k w (DfracOwn 1)) (at level 20) : bi_scope. *)
-(* Notation "k '⤇(KVS)[' idx  ']' -" := *)
-(*   (∃ w, kvs_frag_idx_frac idx k w (DfracOwn 1))%I (at level 20) : bi_scope. *)
-
-(* Definition kvs_frag `{kvsG} (k : Z ) (w : Word) : iProp Σ := ∃ idx, k ⤇(KVS)[ idx ] w. *)
-(* Notation "k '⤇(KVS)' w" := (kvs_frag k w) (at level 20) : bi_scope. *)
-(* Notation "k '⤇(KVS)' -" := (∃ w, kvs_frag k w)%I (at level 20) : bi_scope. *)
-
-(* Notation "●(KVS) m" := (gen_heap_interp (m : kvs_map)) (at level 20) : bi_scope. *)
 
 Section KVS_preamble.
   Context
@@ -548,158 +1020,22 @@ Section KVS_preamble.
   .
 
 
-  Local Lemma kvs_not_elem_of_logical_kvs (lm : kvs_logical_map) (uk mk : Z) ( w : Word ) :
-    ¬ kvs_elem_of_logical_kvs lm uk mk w ->
-    lm !! uk = None ∨
-    ∃ (umap : kvs_user_map), lm !! uk = Some umap ∧ umap !! mk ≠ Some w.
-  Proof.
-    rewrite /kvs_elem_of_logical_kvs.
-    intros H.
-    destruct (lm !! uk) as [umap|] eqn:H' ;[right|left]; auto.
-    exists umap.
-    split; auto.
-    destruct ( umap !! mk ) eqn:Hmk; auto.
-    destruct (decide (w = w0)); simplify_eq; auto.
-    - exfalso; apply H.
-     exists umap; split; auto.
-    - injection; done.
-  Qed.
-
-  Definition kvs_logical_kvs_insert (lm : kvs_logical_map) (uk mk : Z) (w : Word) :=
-   <[uk := (<[ mk := w ]> (default ∅ (lm !! uk))) ]> lm.
-
-  Definition kvs_logical_kvs_delete (lm : kvs_logical_map) (uk mk : Z) :=
-   <[uk := (delete mk (default ∅ (lm !! uk))) ]> lm.
-
-  Lemma kvs_logical_kvs_insert_lookup_eq (lm : kvs_logical_map) (uk mk : Z) (w : Word) (umap : kvs_user_map) :
-    kvs_logical_kvs_insert lm uk mk w !! uk = Some umap ->
-    umap = <[mk := w]> (default ∅ (lm !! uk)).
-  Proof.
-    intros H.
-    rewrite /kvs_logical_kvs_insert in H; simplify_map_eq.
-    done.
-  Qed.
-
-  Lemma kvs_logical_kvs_insert_lookup_ne (lm : kvs_logical_map) (uk uk' mk : Z) (w : Word) (umap : kvs_user_map) :
-    uk ≠ uk' ->
-    kvs_logical_kvs_insert lm uk mk w !! uk' = Some umap ->
-    lm !! uk' = Some umap.
-  Proof.
-    intros Hk H.
-    rewrite /kvs_logical_kvs_insert in H; simplify_map_eq.
-    done.
-  Qed.
-
-  Lemma kvs_logical_kvs_delete_lookup_eq
-    (lm : kvs_logical_map) (uk mk : Z) (umap : kvs_user_map) :
-    kvs_logical_kvs_delete lm uk mk !! uk = Some umap ->
-    umap = delete mk (default ∅ (lm !! uk)).
-  Proof.
-    intros H.
-    rewrite /kvs_logical_kvs_delete in H; simplify_map_eq.
-    done.
-  Qed.
-
-  Lemma kvs_logical_kvs_delete_lookup_ne
-    (lm : kvs_logical_map) (uk uk' mk : Z) (umap : kvs_user_map) :
-    uk ≠ uk' ->
-    kvs_logical_kvs_delete lm uk mk !! uk' = Some umap ->
-    lm !! uk' = Some umap.
-  Proof.
-    intros Hk H.
-    rewrite /kvs_logical_kvs_delete in H; simplify_map_eq.
-    done.
-  Qed.
-
-  (* Definition isKVS *)
-  (*   (a : Addr) (m : kvs_map) (lm : kvs_logical_map) : iProp Σ := *)
-  (*   ⌜ wf_kvs_map m ⌝ ∗ *)
-  (*   ⌜ kvs_synced_logical_kvs m lm ⌝ ∗ *)
-  (*   ●(KVS) m ∗ *)
-  (*   ↪●KVS_USERS lm ∗ *)
-  (*   [∗ map] idx ↦ kw ∈ m, isKVS_entry a idx kw. *)
-
-  (* Definition isKVS_open *)
-  (*   (a : Addr) (m : kvs_map) (lm : kvs_logical_map) (open_idx : nat) : iProp Σ := *)
-  (*   ⌜ wf_kvs_map m ⌝ ∗ *)
-  (*   ⌜ kvs_synced_logical_kvs m lm ⌝ ∗ *)
-  (*   ●(KVS) m ∗ *)
-  (*   ↪●KVS_USERS lm ∗ *)
-  (*   [∗ map] idx ↦ kw ∈ (delete open_idx m), isKVS_entry a idx kw. *)
-
-
-  Lemma NoDup_kvs_keys_update (m : kvs_physical_map) (idx : nat) (k : Z) (w w' : Word) :
-    m !! idx = Some (Some (k, w)) ->
-    NoDup (kvs_keys m) ->
-    NoDup (kvs_keys (<[idx := Some (k, w') ]>m)).
-  Proof.
-    move: idx k w w'.
-    induction m using map_ind; intros idx k w w' Hk Hnodup; first simplify_map_eq.
-    destruct (decide (idx = i)); simplify_map_eq.
-    - rewrite insert_insert_eq.
-      rewrite kvs_keys_insert_Some; auto.
-      rewrite kvs_keys_insert_Some in Hnodup; auto.
-    - rewrite insert_insert_ne; last done.
-      destruct x as [ [k' w''] |].
-      + rewrite kvs_keys_insert_Some in Hnodup; auto.
-        rewrite kvs_keys_insert_Some; simplify_map_eq; auto.
-        apply NoDup_cons in Hnodup as [HkX Hnodup].
-        apply NoDup_cons; split; last (eapply IHm; eauto).
-        intro Hcontra.
-        apply elem_of_kvs_keys in Hcontra as (w0 & idx0 & H0).
-        apply HkX.
-        apply elem_of_kvs_keys; auto.
-        destruct (decide (idx = idx0)); simplify_map_eq.
-        { exists w, idx0; done. }
-        { exists w0, idx0; done. }
-      + rewrite kvs_keys_insert_None in Hnodup; auto.
-        rewrite kvs_keys_insert_None; simplify_map_eq; auto.
-        eapply IHm; eauto.
-  Qed.
-
-  Lemma NoDup_kvs_keys_insert_Some
-    (m : kvs_physical_map) (idx : nat) (k : Z) (w : Word) :
-    k ∉ kvs_keys m ->
-    NoDup (kvs_keys m) ->
-    NoDup (kvs_keys (<[idx:= Some (k, w)]> m)).
-  Proof.
-    move: idx k w.
-    induction m using map_ind; intros idx k w Hk Hnodup.
-    { rewrite kvs_keys_insert_Some; simplify_map_eq; auto.
-      rewrite kvs_keys_empty.
-      apply NoDup_singleton.
-    }
-    destruct (decide (idx = i)); simplify_map_eq.
-    - rewrite insert_insert_eq.
-      rewrite kvs_keys_insert_Some; auto.
-      destruct x as [ [k' w''] |].
-      + rewrite kvs_keys_insert_Some in Hnodup; auto.
-        rewrite kvs_keys_insert_Some in Hk; auto.
-        apply not_elem_of_cons in Hk as [Hkk' Hk].
-        apply NoDup_cons in Hnodup as [Hk' Hnodup].
-        apply NoDup_cons; split; auto.
-      + rewrite kvs_keys_insert_None in Hnodup; auto.
-        rewrite kvs_keys_insert_None in Hk; auto.
-        apply NoDup_cons; split; auto.
-    - rewrite insert_insert_ne; last done.
-      destruct x as [ [k' w''] |].
-      + rewrite kvs_keys_insert_Some in Hnodup; auto.
-        rewrite kvs_keys_insert_Some in Hk; auto.
-        rewrite kvs_keys_insert_Some; simplify_map_eq; auto.
-        apply not_elem_of_cons in Hk as [Hkk' Hk].
-        apply NoDup_cons in Hnodup as [Hk' Hnodup].
-        apply NoDup_cons; split; auto.
-        intro Hcontra.
-        apply elem_of_kvs_keys in Hcontra.
-        destruct Hcontra as (w0&idx0&Hcontra).
-        destruct (decide (idx0 = idx)); simplify_map_eq.
-        apply Hk'.
-        apply elem_of_kvs_keys.
-        eexists _,_;eauto.
-      + rewrite kvs_keys_insert_None in Hnodup; auto.
-        rewrite kvs_keys_insert_None in Hk; auto.
-        rewrite kvs_keys_insert_None; simplify_map_eq; auto.
-  Qed.
+  (* Local Lemma kvs_not_elem_of_logical_kvs (lm : kvs_logical_map) (uk mk : Z) ( w : Word ) : *)
+  (*   ¬ kvs_elem_of_logical_kvs lm uk mk w -> *)
+  (*   lm !! uk = None ∨ *)
+  (*   ∃ (umap : kvs_user_map), lm !! uk = Some umap ∧ umap !! mk ≠ Some w. *)
+  (* Proof. *)
+  (*   rewrite /kvs_elem_of_logical_kvs. *)
+  (*   intros H. *)
+  (*   destruct (lm !! uk) as [umap|] eqn:H' ;[right|left]; auto. *)
+  (*   exists umap. *)
+  (*   split; auto. *)
+  (*   destruct ( umap !! mk ) eqn:Hmk; auto. *)
+  (*   destruct (decide (w = w0)); simplify_eq; auto. *)
+  (*   - exfalso; apply H. *)
+  (*    exists umap; split; auto. *)
+  (*   - injection; done. *)
+  (* Qed. *)
 
   Lemma NoDup_kvs_keys_insert_None
     (m : kvs_physical_map) (idx : nat) :
@@ -785,20 +1121,9 @@ Section KVS_preamble.
     done.
   Qed.
 
-  (* Lemma kvs_initial_map_init_None : *)
-  (* ([∗ map] l↦v ∈ kvs_physical_map_init, pointsto l (DfracOwn 1) v) -∗ *)
-  (* ([∗ map] idx↦_ ∈ kvs_physical_map_init, idx⤇(KVS) NONE). *)
-  (* Proof. *)
-  (*   iIntros "Hkvs_frags". *)
-  (*   iApply (big_sepM_impl with "Hkvs_frags"). *)
-  (*   iModIntro; iIntros (k v Hk) "H". *)
-  (*   apply elem_of_kvs_physical_map_init in Hk; simplify_eq; iFrame. *)
-  (* Qed. *)
-
   Lemma kvs_initial_map_init (b e : Addr) :
     (b + (ASM_SIZEOF_KVS_ENTRY * SIZE_MAP))%a = Some e ->
     ([[b,e]]↦ₐ[[kvs_data]]) -∗
-    (* ([∗ map] idx↦opt_kw ∈ kvs_physical_map_init, idx ⤇(KVS) NONE) -∗ *)
     [∗ map] idx↦kw ∈ kvs_physical_map_init, physical_kvs_entry b idx kw.
   Proof.
     rewrite /kvs_physical_map_init /kvs_data.
@@ -809,14 +1134,6 @@ Section KVS_preamble.
     induction SIZE_MAP; iIntros (k e Hbe) "Hmem"; cbn; first done.
 
     specialize (IHn (S k)).
-    (* iDestruct (big_sepM_insert with "Hfrags") as "[Hf Hfrags]". *)
-    (* { apply not_elem_of_list_to_map. *)
-    (*   intro Hcontra. *)
-    (*   apply list_elem_of_fmap in Hcontra as ([idx opt_kw ] & ? & Hcontra); simplify_eq. *)
-    (*   apply list_elem_of_fmap in Hcontra as (k' & ? & Hcontra); simplify_eq. *)
-    (*   apply elem_of_seq in Hcontra; cbn in *. *)
-    (*   lia. *)
-    (* } *)
     iApply big_sepM_insert.
     { apply not_elem_of_list_to_map.
       intro Hcontra.
@@ -845,689 +1162,7 @@ Section KVS_preamble.
       done.
   Qed.
 
-  Lemma wf_kvs_physical_map_insert (m : kvs_physical_map) (idx : nat) (k : Z) (w : Word) :
-    m !! idx = Some None ->
-    k ∉ kvs_keys m ->
-    wf_kvs_physical_map m ->
-    wf_kvs_physical_map (<[idx:= Some (k, w)]> m).
-  Proof.
-    intros Hidx Hk (Hkvs_dom & Hkvs_unique).
-    split.
-    - rewrite dom_insert_L -Hkvs_dom.
-      assert (idx ∈ dom m).
-      { apply elem_of_dom; eauto. }
-      set_solver.
-    - eapply NoDup_kvs_keys_insert_Some; eauto.
-  Qed.
-
-  Local Lemma kvs_synced_logical_kvs_insert_1
-    (m : kvs_physical_map) ( lm : kvs_logical_map )
-    (idx : nat)
-    (uk mk uk' mk' : Z) (w w' : Word) :
-    let fkey := kvs_full_key uk mk in
-    is_uint16 mk ->
-    m !! idx = Some None ->
-    kvs_synced_logical_kvs m lm ->
-    is_uint16 mk' ->
-    kvs_elem_of_logical_kvs (kvs_logical_kvs_insert lm uk mk w) uk' mk' w' ->
-    kvs_elem_of_kvs (<[idx:= Some (fkey, w)]> m) (kvs_full_key uk' mk') w'.
-  Proof.
-    intros fkey Hwf_full_key Hidx Halloc Hwf_full_key' Hk.
-    destruct Hk as (umap & Huk' & Hmk').
-    destruct (decide (uk = uk')); simplify_map_eq.
-    - apply kvs_logical_kvs_insert_lookup_eq in Huk'; simplify_map_eq.
-      destruct (decide (mk' = mk)) as [Hmk_eq | Hmk_eq]; simplify_map_eq.
-      + eexists idx; simplify_map_eq; done.
-      + specialize (Halloc (uk', mk') w' Hwf_full_key'); cbn in *.
-        rewrite /kvs_elem_of_logical_kvs in Halloc.
-        destruct ( lm !! uk' ) as [umap_uk|] eqn:Hlm; last set_solver+Hmk'.
-        cbn in Hmk'.
-        rewrite Hlm in Halloc.
-        assert (∃ umap : kvs_user_map, Some umap_uk = Some umap
-                                       ∧ umap !! mk' = Some w') as IH.
-        { exists umap_uk; split; auto. }
-        apply Halloc in IH.
-        destruct IH as (idx' & Hk).
-        destruct (decide (idx = idx')); simplify_map_eq; cbn in *; auto.
-        by eexists idx'; simplify_map_eq.
-    - apply kvs_logical_kvs_insert_lookup_ne in Huk'; auto; simplify_map_eq.
-      assert (∃ umap : kvs_user_map, lm !! uk' = Some umap ∧ umap !! mk' = Some w') as IH.
-      { exists umap; split; auto. }
-      specialize (Halloc (uk', mk') w' Hwf_full_key'); cbn in *.
-      rewrite /kvs_elem_of_logical_kvs in Halloc.
-      apply Halloc in IH.
-      destruct IH as (idx' & Hk).
-      destruct (decide (idx = idx')); simplify_map_eq; cbn in *; auto.
-      by eexists idx'; simplify_map_eq.
-  Qed.
-
-  Local Lemma kvs_synced_logical_kvs_insert_2
-    (m : kvs_physical_map) ( lm : kvs_logical_map )
-    (idx : nat)
-    (uk mk uk' mk' : Z) (w w' : Word) :
-    let fkey := kvs_full_key uk mk in
-    is_uint16 mk ->
-    m !! idx = Some None ->
-    fkey ∉ kvs_keys m ->
-    kvs_synced_logical_kvs m lm ->
-    is_uint16 mk' ->
-    kvs_elem_of_kvs (<[idx:= Some (fkey, w)]> m) (kvs_full_key uk' mk') w' ->
-    kvs_elem_of_logical_kvs (kvs_logical_kvs_insert lm uk mk w) uk' mk' w'.
-  Proof.
-    intros fkey Hwf_full_key Hidx Hkfree Halloc Hwf_full_key' Hk.
-    specialize (Halloc (uk', mk') w' Hwf_full_key') as IH.
-    destruct Hk as (idx' & Hk).
-    destruct (decide (idx = idx')); simplify_map_eq; cbn in *; auto.
-    - apply kvs_full_key_inj in Hk as [ -> -> ]; eauto.
-      rewrite /kvs_logical_kvs_insert;simplify_map_eq.
-      rewrite /kvs_elem_of_logical_kvs;simplify_map_eq.
-      exists (<[mk':=w']> (default ∅ (lm !! uk'))); split; auto.
-      by simplify_map_eq.
-    - rewrite /kvs_logical_kvs_insert;simplify_map_eq.
-      rewrite /kvs_elem_of_logical_kvs;simplify_map_eq.
-      assert ( kvs_elem_of_kvs m (kvs_full_key uk' mk') w' ) as IHm.
-      { eexists; eauto. }
-      destruct (decide (uk = uk')); simplify_map_eq.
-      + destruct (decide (mk = mk')); simplify_map_eq.
-        * apply (iffLRn (elem_of_kvs_keys m fkey)) in Hkfree.
-          exfalso; apply Hkfree; eexists _,_; eauto.
-        * apply IH in IHm as (umap & Humap & Humap').
-          by eexists ; split; eauto; simplify_map_eq.
-      + apply IH in IHm as (umap & Humap & Humap').
-        eexists ; split; eauto.
-  Qed.
-
-  Lemma kvs_synced_logical_kvs_insert (m : kvs_physical_map) ( lm : kvs_logical_map ) (idx : nat) (uk mk : Z) (w : Word) :
-    let fkey := kvs_full_key uk mk in
-    is_uint16 mk ->
-    m !! idx = Some None ->
-    fkey ∉ kvs_keys m ->
-    kvs_synced_logical_kvs m lm ->
-    kvs_synced_logical_kvs (<[idx:=Some (fkey, w)]> m) ( kvs_logical_kvs_insert lm uk mk w).
-  Proof.
-    intros fkey Hwf_full_key Hidx Hk_free Halloc.
-    intros [uk' mk'] Hwf_full_key'.
-    cbn.
-    split; intros Hk.
-    - eapply kvs_synced_logical_kvs_insert_1; eauto.
-    - eapply kvs_synced_logical_kvs_insert_2; eauto.
-  Qed.
-
-  Lemma wf_kvs_physical_map_update (m : kvs_physical_map) (idx : nat) (k : Z) (w : Word) :
-    (∃ w', m !! idx = Some (Some (k, w'))) ->
-    wf_kvs_physical_map m ->
-    wf_kvs_physical_map (<[idx:= Some (k, w)]> m).
-  Proof.
-    intros [w' Hidx] (Hkvs_dom & Hkvs_unique).
-    split.
-    - rewrite dom_insert_L -Hkvs_dom.
-      assert (idx ∈ dom m).
-      { apply elem_of_dom; eauto. }
-      set_solver.
-    - eapply NoDup_kvs_keys_update; eauto.
-  Qed.
-
-  (* Lemma kvs_frag_kvs_frag_idx (k : Z) (w : Word) : *)
-  (*   k ⤇(KVS) w -∗ ∃ idx, k ⤇(KVS)[idx] w. *)
-  (* Proof. rewrite /kvs_frag; iIntros "?"; done. Qed. *)
-
-  (* Lemma kvs_frag_idx_kvs_frag (k : Z) (w : Word) (idx : nat) : *)
-  (*   k ⤇(KVS)[idx] w -∗ k ⤇(KVS) w. *)
-  (* Proof. rewrite /kvs_frag; iIntros "$".  Qed. *)
-
-  (* Lemma kvs_auth_insert (a : Addr) (m : kvs_physical_map) (idx : nat) (k : Z) (w : Word) : *)
-  (*   ●(KVS) m -∗ idx ⤇(KVS) NONE *)
-  (*   ==∗ *)
-  (*   ●(KVS) (<[idx:= Some (k, w)]> m) ∗ k ⤇(KVS)[ idx ] w. *)
-  (* Proof. *)
-  (*   iIntros "Hkvs_auth Hkvs_frag". *)
-  (*   by iMod (gen_heap_update m idx _ (Some (k,w)) with "Hkvs_auth Hkvs_frag") as "[$ $]". *)
-  (* Qed. *)
-
-  (* Lemma kvs_auth_update (a : Addr) (m : kvs_physical_map) (idx : nat) (k k' : Z) (w w' : Word) : *)
-  (*   ●(KVS) m -∗ k ⤇(KVS)[ idx ] w *)
-  (*   ==∗ *)
-  (*   ●(KVS) (<[idx:= Some (k', w')]> m) ∗ k' ⤇(KVS)[ idx ] w'. *)
-  (* Proof. *)
-  (*   iIntros "Hkvs_auth Hkvs_frag". *)
-  (*   by iMod (gen_heap_update m idx _ (Some (k',w')) with "Hkvs_auth Hkvs_frag") as "[$ $]". *)
-  (* Qed. *)
-
-  (* Lemma kvs_auth_delete (a : Addr) (m : kvs_physical_map) (idx : nat) (k : Z) (w : Word) : *)
-  (*   ●(KVS) m -∗ k ⤇(KVS)[ idx ] w *)
-  (*   ==∗ *)
-  (*   ●(KVS) (<[idx:= None]> m) ∗ idx ⤇(KVS) NONE. *)
-  (* Proof. *)
-  (*   iIntros "Hkvs_auth Hkvs_frag". *)
-  (*   by iMod (gen_heap_update m idx _ None with "Hkvs_auth Hkvs_frag") as "[$ $]". *)
-  (* Qed. *)
-
-  (* Lemma kvs_frag_idx_dupl_false idx k k' w w' : *)
-  (*   k ⤇(KVS)[ idx ] w -∗ k' ⤇(KVS)[ idx ] w' -∗ False. *)
-  (* Proof. *)
-  (*   iIntros "H1 H2". *)
-  (*   iDestruct (pointsto_valid_2 with "H1 H2") as %?. *)
-  (*   destruct H; eapply dfrac_full_exclusive in H; auto. *)
-  (* Qed. *)
-
-  (* Lemma kvs_valid_None (m : kvs_physical_map) (idx : nat) : *)
-  (*   ●(KVS) m -∗ *)
-  (*   idx ⤇(KVS) NONE -∗ *)
-  (*   ⌜ m !! idx = Some None ⌝. *)
-  (* Proof. *)
-  (*   iIntros "Hkvs_auth Hk". *)
-  (*   by iDestruct (gen_heap_valid with "Hkvs_auth Hk") as "%Hidx'". *)
-  (* Qed. *)
-
-  (* Lemma kvs_valid (m : kvs_physical_map) (idx : nat) (k : Z) (w : Word) : *)
-  (*   ●(KVS) m -∗ *)
-  (*   k ⤇(KVS)[idx] w -∗ *)
-  (*   ⌜ m !! idx = Some (Some (k, w)) ⌝. *)
-  (* Proof. *)
-  (*   iIntros "Hkvs_auth Hk". *)
-  (*   by iDestruct (gen_heap_valid with "Hkvs_auth Hk") as "%Hidx'". *)
-  (* Qed. *)
-
-  (* Lemma isKVS_valid (m : kvs_physical_map) (lm : kvs_logical_map) (a : Addr) (idx : nat) (k : Z) (w : Word) : *)
-  (*   isKVS a m lm -∗ *)
-  (*   k ⤇(KVS)[idx] w -∗ *)
-  (*   ⌜ m !! idx = Some (Some (k, w)) ⌝. *)
-  (* Proof. *)
-  (*   iIntros "(%Hwf_kvs & _ & Hkvs_auth & _) Hk". *)
-  (*   by iDestruct (kvs_valid with "Hkvs_auth Hk") as "%Hidx'". *)
-  (* Qed. *)
-
-  (* Lemma isKVS_valid_None (m : kvs_physical_map) (lm : kvs_logical_map) (a : Addr) (idx : nat) : *)
-  (*   isKVS a m lm -∗ *)
-  (*   idx ⤇(KVS) NONE -∗ *)
-  (*   ⌜ m !! idx = Some None ⌝. *)
-  (* Proof. *)
-  (*   iIntros "(%Hwf_kvs & _ & Hkvs_auth & _) Hk". *)
-  (*   by iDestruct (kvs_valid_None with "Hkvs_auth Hk") as "%Hidx'". *)
-  (* Qed. *)
-
-  (* Lemma isKVS_open_valid (m : kvs_physical_map) (lm : kvs_logical_map) (a : Addr) (idx idx' : nat) (k : Z) (w : Word) : *)
-  (*   isKVS_open a m lm idx' -∗ *)
-  (*   k ⤇(KVS)[idx] w -∗ *)
-  (*   ⌜ m !! idx = Some (Some (k, w)) ⌝. *)
-  (* Proof. *)
-  (*   iIntros "(%Hwf_kvs & _ & Hkvs_auth & _) Hk". *)
-  (*   by iDestruct (kvs_valid with "Hkvs_auth Hk") as "%Hidx'". *)
-  (* Qed. *)
-
-  (* Lemma isKVS_open_valid_None (m : kvs_physical_map) (lm : kvs_logical_map) (a : Addr) (idx idx' : nat) : *)
-  (*   isKVS_open a m lm idx' -∗ *)
-  (*   idx ⤇(KVS) NONE -∗ *)
-  (*   ⌜ m !! idx = Some None ⌝. *)
-  (* Proof. *)
-  (*   iIntros "(%Hwf_kvs & _ & Hkvs_auth & _) Hk". *)
-  (*   by iDestruct (kvs_valid_None with "Hkvs_auth Hk") as "%Hidx'". *)
-  (* Qed. *)
-
-  (* Lemma open_isKVS_kvs_frag_idx *)
-  (*   (b : Addr) (m : kvs_physical_map) (lm : kvs_logical_map) *)
-  (*   (idx : nat) (k : Z) (w : Word) : *)
-  (*   isKVS b m lm ∗ *)
-  (*   k ⤇(KVS)[idx] w -∗ *)
-  (*   isKVS_open b m lm idx ∗ *)
-  (*   isKVS_entry b idx (Some (k, w)) ∗ *)
-  (*   k ⤇(KVS)[idx] w. *)
-  (* Proof. *)
-  (*   iIntros "( (%Hwf_kvs & %Hwf_alloc & Hkvs_auth & Halloc & HKVS) & Hk)". *)
-  (*   iDestruct (gen_heap_valid with "Hkvs_auth Hk") as "%Hidx'". *)
-  (*   rewrite -{2}(insert_id m idx (Some (k,w))); last done. *)
-  (*   iDestruct (big_sepM_insert_delete with "HKVS") as "[Hkvs_entry HKVS]". *)
-  (*   iFrame; eauto. *)
-  (* Qed. *)
-
-  (* Lemma isKVS_indom_idx (m : kvs_physical_map) (lm : kvs_logical_map) (a : Addr) (idx : nat) : *)
-  (*   idx ∈ dom m -> *)
-  (*   isKVS a m lm -∗ *)
-  (*   ⌜ 0 <= idx < SIZE_MAP ⌝. *)
-  (* Proof. *)
-  (*   iIntros (Hm_idx) "(%Hwf_kvs & _)"; iPureIntro. *)
-  (*   by eapply wf_kvs_indom_idx. *)
-  (* Qed. *)
-
-  (* Lemma isKVS_open_indom_idx (m : kvs_physical_map) (lm : kvs_logical_map) (a : Addr) (idx idx' : nat) : *)
-  (*   idx ∈ dom m -> *)
-  (*   isKVS_open a m lm idx' -∗ *)
-  (*   ⌜ 0 <= idx < SIZE_MAP ⌝. *)
-  (* Proof. *)
-  (*   iIntros (Hm_idx) "(%Hwf_kvs & _)"; iPureIntro. *)
-  (*   by eapply wf_kvs_indom_idx. *)
-  (* Qed. *)
-
-  (* Lemma open_isKVS_kvs_frag_idx_diff *)
-  (*   (b : Addr) (m : kvs_physical_map) (lm : kvs_logical_map) (idx idx' : nat) (k : Z) (w : Word): *)
-  (*   0 <= idx' < SIZE_MAP -> *)
-  (*   idx ≠ idx' -> *)
-  (*   isKVS b m lm ∗ *)
-  (*   k ⤇(KVS)[ idx ] w -∗ *)
-  (*   ∃ opt_kw', *)
-  (*     k ⤇(KVS)[ idx ] w ∗ *)
-  (*     isKVS_open b m lm idx' ∗ *)
-  (*     ⌜ m !! idx' = Some opt_kw' ⌝ ∗ *)
-  (*     isKVS_entry b idx' opt_kw' ∗ *)
-  (*     ⌜ match opt_kw' with | Some kw' => k ≠ kw'.1 | None => True end ⌝. *)
-  (* Proof. *)
-  (*   iIntros (Hidx' Hidx_ne) "( (%Hwf_kvs & %Hwf_alloc & Hkvs_auth & Halloc & HKVS) & Hk)". *)
-  (*   iDestruct (kvs_valid with "Hkvs_auth Hk") as "%Hm_idx". *)
-  (*   pose proof (wf_kvs_is_Some _ _ Hwf_kvs Hidx') as [ opt_kw' Hm_idx' ]. *)
-  (*   iExists opt_kw'. *)
-  (*   rewrite -{2}(insert_id m idx' opt_kw'); last done. *)
-  (*   iDestruct (big_sepM_insert_delete with "HKVS") as "[ Hk' HKVS]". *)
-  (*   iFrame "∗%". *)
-  (*   iPureIntro. *)
-  (*   destruct opt_kw' as [ [k' w'] |]; auto. *)
-  (*   pose proof (wf_kvs_neq _ _ _ _ _ _ _ Hwf_kvs Hidx_ne Hm_idx Hm_idx') as Hkk'. *)
-  (*   done. *)
-  (* Qed. *)
-
-  (* Lemma open_isKVS_not_alloc *)
-  (*   (b : Addr) (m : kvs_physical_map) (lm : kvs_logical_map) (umap : kvs_user_map) *)
-  (*   (idx : nat) (ku kn : Z) : *)
-  (*   let fkey := kvs_full_key ku kn in *)
-  (*   is_uint16 kn -> *)
-  (*   (0 ≤ idx < SIZE_MAP)%Z → *)
-  (*   kn ∉ dom umap → *)
-  (*   isKVS b m lm -∗ *)
-  (*   ku ↦(KVS_USER) umap -∗ *)
-  (*   ∃ opt_kwidx, *)
-  (*     ⌜ m !! idx = Some opt_kwidx ⌝ ∗ *)
-  (*     isKVS_open b m lm idx ∗ *)
-  (*     ku ↦(KVS_USER) umap ∗ *)
-  (*     isKVS_entry b idx opt_kwidx ∗ *)
-  (*     ⌜ match opt_kwidx with | Some kwidx => kwidx.1 ≠ fkey | None => True end ⌝. *)
-  (* Proof. *)
-  (*   intros fkey Hwf_full_key Hidx Hs'. *)
-  (*   iIntros "(%Hwf_kvs & %Hwf_alloc & Hkvs_auth & Halloc  & HKVS) Hk". *)
-  (*   iDestruct ( kvs_logical_kvs_valid with "Halloc Hk" ) as "%Hss'". *)
-  (*   assert (fkey ∉ kvs_keys m) as Hfkey_not_allocated. *)
-  (*   { apply not_elem_of_dom in Hs'. *)
-  (*     intro Hcontra. *)
-  (*     apply elem_of_kvs_keys in Hcontra as (idx'&w&?). *)
-  (*     ospecialize (Hwf_alloc (ku, kn) w Hwf_full_key). *)
-  (*     cbn in Hwf_alloc. *)
-  (*     assert ( kvs_elem_of_kvs m (kvs_full_key ku kn) w ) as Helem. *)
-  (*     { eexists; eauto. } *)
-  (*     apply Hwf_alloc in Helem. *)
-  (*     destruct Helem as (?&?&?); simplify_map_eq. *)
-  (*   } *)
-  (*   iFrame. *)
-  (*   assert ( is_Some (m !! idx) ) as [ opt_kwidx Hm_idx]. *)
-  (*   { apply wf_kvs_is_Some; auto; lia. } *)
-  (*   rewrite -{1}(insert_id m idx opt_kwidx); last done. *)
-  (*   iDestruct (big_sepM_insert_delete with "HKVS") as "[Hkvs_entry HKVS]". *)
-  (*   iFrame "∗%". *)
-  (*   iPureIntro. *)
-  (*   destruct opt_kwidx as [ [ kidx widx ]|]; auto. *)
-  (*   cbn. *)
-  (*   assert ( kidx ∈ kvs_keys m ) as Hkidx by (apply elem_of_kvs_keys; eauto). *)
-  (*   set_solver. *)
-  (* Qed. *)
-
-  (* Lemma open_isKVS *)
-  (*   (b : Addr) (m : kvs_physical_map) (lm : kvs_logical_map) *)
-  (*   (idx : nat) : *)
-  (*   (0 ≤ idx < SIZE_MAP)%Z → *)
-  (*   isKVS b m lm -∗ *)
-  (*   ∃ opt_kwidx, *)
-  (*     ⌜ m !! idx = Some opt_kwidx ⌝ ∗ *)
-  (*     isKVS_open b m lm idx ∗ *)
-  (*     isKVS_entry b idx opt_kwidx. *)
-  (* Proof. *)
-  (*   intros Hidx. *)
-  (*   iIntros "(%Hwf_kvs & %Hwf_alloc & Hkvs_auth & Halloc & HKVS)". *)
-  (*   iFrame. *)
-  (*   assert ( is_Some (m !! idx) ) as [ opt_kwidx Hm_idx]. *)
-  (*   { apply wf_kvs_is_Some; auto; lia. } *)
-  (*   rewrite -{1}(insert_id m idx opt_kwidx); last done. *)
-  (*   iDestruct (big_sepM_insert_delete with "HKVS") as "[Hkvs_entry HKVS]". *)
-  (*   iFrame "∗%". *)
-  (* Qed. *)
-
-  (* Lemma close_isKVS *)
-  (*   (b : Addr) (m : kvs_physical_map) (lm : kvs_logical_map) (idx : nat) (opt_kwidx : kvs_entry): *)
-  (*   m !! idx = Some opt_kwidx -> *)
-  (*   isKVS_open b m lm idx ∗ *)
-  (*   isKVS_entry b idx opt_kwidx -∗ *)
-  (*   isKVS b m lm. *)
-  (* Proof. *)
-  (*   iIntros (Hidx) "[(%Hwf_kvs & %Hwf_alloc & Hkvs_auth & Halloc & HKVS) Hkvs_entry]"; cbn. *)
-  (*   iDestruct (big_sepM_delete with "[$HKVS $Hkvs_entry]") as "HKVS"; eauto. *)
-  (*   iFrame; eauto. *)
-  (* Qed. *)
-
-  Lemma NoDup_kvs_keys_elem_of m idx uk mk w idx' uk' mk' w' :
-    let f := kvs_full_key uk mk in
-    let f' := kvs_full_key uk' mk' in
-    NoDup (kvs_keys m) ->
-    idx ≠ idx' ->
-    m !! idx = Some (Some (f, w)) ->
-    m !! idx' = Some (Some (f', w')) ->
-    uk' ≠ uk ∨ mk' ≠ mk.
-  Proof.
-    intros f f'.
-    induction m using map_ind; intros Hnodup Hidx_ne Hm_idx Hm_idx'; first set_solver.
-    simplify_map_eq.
-    destruct x as [ [kx wx] |]; cycle 1.
-    - rewrite kvs_keys_insert_None in Hnodup; auto.
-      assert (idx ≠ i) as Hidx_i_ne by (intro; simplify_map_eq; done).
-      assert (idx' ≠ i) as Hidx'_i_ne by (intro; simplify_map_eq; done).
-      simplify_map_eq.
-      auto.
-    - rewrite kvs_keys_insert_Some in Hnodup; auto.
-      apply NoDup_cons in Hnodup as [Hkx_not_elem_kvs_keys Hnodup].
-      destruct (decide (idx = i)); simplify_map_eq.
-      + (* idx = i *)
-        assert (f' ∈ kvs_keys m) as Hf'.
-        { apply elem_of_kvs_keys; eexists _,_; eauto. }
-        destruct (decide (uk' = uk)); simplify_eq; [right|left]; auto.
-        destruct (decide (mk' = mk)); simplify_eq; auto.
-      + destruct (decide (idx' = i)); simplify_map_eq.
-        * (* idx ≠ i ∧ idx' = i *)
-          assert (f ∈ kvs_keys m) as Hf.
-          { apply elem_of_kvs_keys; eexists _,_; eauto. }
-          destruct (decide (uk' = uk)); simplify_eq; [right|left]; auto.
-          destruct (decide (mk' = mk)); simplify_eq; auto.
-        * (* idx ≠ i ∧ idx' ≠ i *)
-          eapply IHm; eauto.
-  Qed.
-
-
-  Lemma kvs_synced_logical_kvs_update
-    (m : kvs_physical_map) (lm : kvs_logical_map) (idx : nat) (uk mk : Z) (w : Word) :
-    let k := kvs_full_key uk mk in
-    NoDup (kvs_keys m) ->
-    is_uint16 mk ->
-    (∃ w', m !! idx = Some ( Some (k, w'))) ->
-    kvs_synced_logical_kvs m lm ->
-    kvs_synced_logical_kvs (<[idx:= Some (k, w)]> m) (kvs_logical_kvs_insert lm uk mk w).
-  Proof.
-    intros k.
-    intros Hnodup Hwf [w' Hidx] Halloc [ku kn] w'' Hwf'.
-    specialize (Halloc (ku, kn) w'' Hwf'); cbn in *.
-    split; intros Hk.
-    - rewrite /kvs_elem_of_logical_kvs in Hk.
-      destruct Hk as (umap & Hlm & Hkn).
-      destruct (decide (ku = uk)); simplify_map_eq.
-      + apply kvs_logical_kvs_insert_lookup_eq in Hlm; simplify_eq.
-        destruct (decide (kn = mk)); simplify_map_eq.
-        * eexists idx; simplify_map_eq; done.
-        * assert ( kvs_elem_of_kvs m (kvs_full_key uk kn) w'' ) as (idx'&?).
-          { apply Halloc. eexists;split;eauto.
-            destruct (lm !! uk) eqn:Hlm; cbn;eauto.
-            cbn in *;set_solver.
-          }
-          eexists idx'.
-          destruct (decide (idx = idx')); simplify_map_eq; cbn in *.
-          ** rewrite Hidx in H; simplify_map_eq.
-             apply kvs_full_key_inj in H as [? ?]; eauto; simplify_eq.
-          ** by simplify_map_eq.
-      + apply kvs_logical_kvs_insert_lookup_ne in Hlm; simplify_eq; auto.
-        assert ( kvs_elem_of_logical_kvs lm ku kn w'') as Hk'.
-        { eexists ; split; eauto. }
-        eapply Halloc in Hk' as (idx' & Hk).
-        destruct (decide (idx = idx')); simplify_map_eq; cbn in *.
-        ** rewrite Hidx in Hk; simplify_map_eq.
-           apply kvs_full_key_inj in Hk as [? ?]; eauto; simplify_eq.
-        ** by eexists idx'; simplify_map_eq.
-    - destruct Hk as (idx' & Hk).
-      destruct (decide (idx = idx')); simplify_map_eq; cbn in *.
-      + apply kvs_full_key_inj in Hk as [? ?]; eauto; simplify_eq.
-        rewrite /kvs_elem_of_logical_kvs /kvs_logical_kvs_insert.
-        destruct (lm !! ku) as [umap|] eqn:Humap ; simplify_map_eq.
-        * by eexists; split; eauto; simplify_map_eq.
-        * by eexists; split; eauto; simplify_map_eq.
-      + assert ( kvs_elem_of_logical_kvs lm ku kn w'' ) as (umap&Hlm&Hkn).
-        { apply Halloc; eexists; eauto. }
-        rewrite /kvs_elem_of_logical_kvs /kvs_logical_kvs_insert.
-        destruct (decide (uk = ku)); simplify_map_eq; cycle 1.
-        * eexists; split; eauto.
-        * destruct (decide (kn = mk)); simplify_map_eq.
-          ** eexists; split; eauto.
-             subst k.
-             eapply (NoDup_kvs_keys_elem_of m idx ku mk _ idx' ku mk) in Hnodup; eauto.
-             destruct Hnodup as [|]; done.
-          ** by eexists; split; eauto; simplify_map_eq.
-  Qed.
-
-  (* Lemma isKVS_open_update *)
-  (*   (a : Addr) (m : kvs_physical_map) (lm : kvs_logical_map) (umap : kvs_user_map) *)
-  (*   (idx : nat) (uk mk : Z) (w w' : Word) : *)
-  (*   let k := kvs_full_key uk mk in *)
-  (*   is_uint16 mk -> *)
-  (*   isKVS_open a m lm idx -∗ *)
-  (*   k ⤇(KVS)[ idx ] w -∗ *)
-  (*   uk ↦(KVS_USER) umap *)
-  (*   ==∗ *)
-  (*   isKVS_open a (<[idx:= Some (k, w')]> m) (kvs_logical_kvs_insert lm uk mk w') idx ∗ *)
-  (*   k ⤇(KVS)[ idx ] w' ∗ *)
-  (*   uk ↦(KVS_USER) ( <[mk:=w']> umap ) *)
-  (* . *)
-  (* Proof. *)
-  (*   intros k Hwf. *)
-  (*   iIntros "(%Hwf_kvs & %Hwf_alloc & Hkvs_auth & Halloc & HKVS) Hk Humap". *)
-  (*   iDestruct (kvs_valid with "Hkvs_auth Hk") as "%Hm_idx". *)
-  (*   iDestruct (kvs_logical_kvs_valid with "Halloc Humap") as "%Hvalid". *)
-  (*   iMod (kvs_auth_update a m idx _ k _ w' with "Hkvs_auth Hk") as "[$ $]". *)
-  (*   iMod (kvs_logical_kvs_update uk lm umap (<[mk:=w']> umap) with "Halloc Humap") as "[Halloc_auth Halloc_frag]". *)
-  (*   eapply (kvs_synced_logical_kvs_update _ _ _ _ _ w') in Hwf_alloc; eauto. *)
-  (*   2: { by destruct Hwf_kvs. } *)
-  (*   eapply (wf_kvs_physical_map_update _ _ _ w') in Hwf_kvs; eauto. *)
-  (*   rewrite delete_insert_eq. *)
-  (*   iFrame "∗ %". *)
-  (*   by rewrite /kvs_logical_kvs_insert Hvalid /=. *)
-  (* Qed. *)
-
-  (* Lemma isKVS_open_insert *)
-  (*   (a : Addr) (m : kvs_physical_map) (lm : kvs_logical_map) *)
-  (*   (umap : kvs_user_map) (idx : nat) (ku kn : Z) (w : Word) : *)
-  (*   let k := kvs_full_key ku kn in *)
-  (*   kn ∉ dom umap → *)
-  (*   is_uint16 kn -> *)
-  (*   isKVS_open a m lm idx -∗ *)
-  (*   ku ↦(KVS_USER) umap -∗ *)
-  (*   idx ⤇(KVS) NONE *)
-  (*   ==∗ *)
-  (*   isKVS_open a (<[idx:= Some (k, w)]> m) (kvs_logical_kvs_insert lm ku kn w) idx ∗ *)
-  (*   ku ↦(KVS_USER) (<[ kn := w ]> umap) ∗ *)
-  (*   k ⤇(KVS)[ idx ] w. *)
-  (* Proof. *)
-  (*   intro k. *)
-  (*   iIntros (Hs' Hwf_kvs_full_key) *)
-  (*     "(%Hwf_kvs & %Hwf_alloc & Hkvs_auth & Halloc_auth & HKVS) Halloc_frag Hk". *)
-  (*   iDestruct (kvs_logical_kvs_valid with "Halloc_auth Halloc_frag") as "%Hvalid". *)
-  (*   iDestruct (kvs_valid_None with "Hkvs_auth Hk") as "%Hm_idx". *)
-  (*   iMod (kvs_auth_insert a m idx k w with "Hkvs_auth Hk") as "[$ $]". *)
-  (*   iMod (kvs_logical_kvs_update ku lm umap (<[kn:=w]> umap) with "Halloc_auth Halloc_frag") as "[Halloc_auth Halloc_frag]". *)
-  (*   rewrite /kvs_synced_logical_kvs in Hwf_alloc. *)
-  (*   assert (k ∉ kvs_keys m) as Hk_not_allocated. *)
-  (*   { apply not_elem_of_dom in Hs'. *)
-  (*     intro Hcontra. *)
-  (*     apply elem_of_kvs_keys in Hcontra as (idx'&w'&?). *)
-  (*     ospecialize (Hwf_alloc (ku, kn) w' Hwf_kvs_full_key). *)
-  (*     cbn in Hwf_alloc. *)
-  (*     assert ( kvs_elem_of_kvs m (kvs_full_key ku kn) w' ) as Helem. *)
-  (*     { eexists; eauto. } *)
-  (*     apply Hwf_alloc in Helem. *)
-  (*     destruct Helem as (?&?&?); simplify_map_eq. *)
-  (*   } *)
-  (*   eapply (wf_kvs_physical_map_insert _ _ _ w) in Hwf_kvs; eauto. *)
-  (*   eapply (kvs_synced_logical_kvs_insert _ _ _ _ _ w) in Hwf_alloc; eauto. *)
-  (*   rewrite delete_insert_eq. *)
-  (*   subst k. *)
-  (*   iFrame "∗ %". *)
-  (*   by rewrite /kvs_logical_kvs_insert Hvalid /=. *)
-  (* Qed. *)
-
-  Local Lemma kvs_synced_logical_kvs_delete_1
-    (m : kvs_physical_map) (lm : kvs_logical_map) (idx : nat) (uk mk uk' mk' : Z) (w w' : Word) :
-    let fkey := kvs_full_key uk mk in
-    is_uint16 mk ->
-    m !! idx = Some (Some (fkey, w)) ->
-    kvs_synced_logical_kvs m lm ->
-    is_uint16 mk' ->
-    kvs_elem_of_logical_kvs (kvs_logical_kvs_delete lm uk mk) uk' mk' w' ->
-    kvs_elem_of_kvs (<[idx:= None]> m) (kvs_full_key uk' mk') w'.
-  Proof.
-    intros fkey Hwf_full_key Hidx Halloc Hwf_full_key' Hk.
-    destruct Hk as (umap & Huk' & Hmk').
-    destruct (decide (uk = uk')); simplify_map_eq.
-    - apply kvs_logical_kvs_delete_lookup_eq in Huk'; simplify_map_eq.
-      assert ( mk ≠ mk' ) as Hmk_eq ; simplify_map_eq.
-      { intro; simplify_map_eq. }
-        destruct ( lm !! uk' ) as [umap_uk|] eqn:Hlm ; last set_solver+Hmk'.
-      cbn in *.
-      assert ( kvs_elem_of_logical_kvs lm uk' mk' w') as Helem.
-      { eexists; split;eauto. }
-      specialize (Halloc (uk', mk') w' Hwf_full_key'); cbn in *.
-      apply Halloc in Helem as (idx'&Hidx').
-      eexists idx'.
-      destruct (decide (idx = idx')); simplify_map_eq; cbn in *; auto.
-      rewrite Hidx in Hidx'; simplify_map_eq.
-      apply kvs_full_key_inj in Hidx' as [_ ->]; eauto; done.
-    - apply kvs_logical_kvs_delete_lookup_ne in Huk'; auto; simplify_map_eq.
-      assert (∃ umap : kvs_user_map, lm !! uk' = Some umap ∧ umap !! mk' = Some w') as IH.
-      { exists umap; split; auto. }
-      apply (Halloc (uk', mk') w' Hwf_full_key') in IH as (idx'&Hidx').
-      destruct (decide (idx = idx')); simplify_map_eq; cbn in *; auto.
-      * rewrite Hidx in Hidx'; simplify_map_eq.
-        apply kvs_full_key_inj in Hidx' as [-> ->] ;eauto; done.
-      * by exists idx'; simplify_map_eq.
-  Qed.
-
-  Local Lemma kvs_synced_logical_kvs_delete_2
-    (m : kvs_physical_map) (lm : kvs_logical_map) (idx : nat) (uk mk uk' mk' : Z) (w w' : Word) :
-    let fkey := kvs_full_key uk mk in
-    is_uint16 mk ->
-    m !! idx = Some (Some (fkey, w)) ->
-    NoDup (kvs_keys m) ->
-    kvs_synced_logical_kvs m lm ->
-    is_uint16 mk' ->
-    kvs_elem_of_kvs (<[idx:= None]> m) (kvs_full_key uk' mk') w' ->
-    kvs_elem_of_logical_kvs (kvs_logical_kvs_delete lm uk mk) uk' mk' w'.
-  Proof.
-    intros fkey Hwf_full_key Hidx Hnodup Halloc Hwf_full_key' Hk.
-    specialize (Halloc (uk', mk') w' Hwf_full_key') as IH'.
-    cbn in *.
-    destruct Hk as (idx' & Hk).
-
-    destruct (decide (idx = idx')); simplify_map_eq; cbn in *; auto.
-    assert (kvs_elem_of_kvs m (kvs_full_key uk' mk') w') as IHm'.
-    { eexists; eauto. }
-
-    apply IH' in IHm' as (umap' & Humap' & Hmk'_in_umap').
-    assert (kvs_full_key uk mk ∈ kvs_keys m) as IHm.
-    { apply elem_of_kvs_keys; eexists _,_; eauto. }
-    rewrite /kvs_logical_kvs_delete.
-    destruct (decide (uk = uk')); simplify_map_eq; cycle 1.
-    { exists umap'; split; simplify_map_eq;eauto. }
-    eexists (delete mk umap'); split; simplify_map_eq; eauto.
-    destruct (decide (mk = mk')); simplify_map_eq; try done.
-
-    eapply (NoDup_kvs_keys_elem_of m idx uk' mk' _ idx' uk' mk') in Hnodup; eauto.
-    destruct Hnodup as [ | ]; done.
-  Qed.
-
-  Lemma kvs_synced_logical_kvs_delete (m : kvs_physical_map) (lm : kvs_logical_map) (idx : nat) (uk mk : Z) (w : Word) :
-    let fkey := kvs_full_key uk mk in
-    NoDup (kvs_keys m) ->
-    is_uint16 mk ->
-    m !! idx = Some (Some (fkey, w)) ->
-    kvs_synced_logical_kvs m lm ->
-    kvs_synced_logical_kvs (<[idx:=None]> m) (kvs_logical_kvs_delete lm uk mk).
-  Proof.
-    intros fkey Hnodup Hwf_full_key Hidx Halloc.
-    intros [uk' mk'] Hwf_full_key'.
-    cbn.
-    split; intros Hk.
-    - eapply (kvs_synced_logical_kvs_delete_1 m lm idx uk mk uk' mk'); eauto.
-    - eapply (kvs_synced_logical_kvs_delete_2 m lm idx uk mk uk' mk'); eauto.
-  Qed.
-
-  Lemma NoDup_kvs_keys_delete
-    (m : kvs_physical_map) (idx : nat)  :
-    NoDup (kvs_keys m) ->
-    NoDup (kvs_keys (<[idx:=None]> m)).
-  Proof.
-    generalize dependent idx.
-    induction m using map_ind; intros idx Hnodup; first simplify_map_eq.
-    { rewrite kvs_keys_insert_None; auto. }
-    destruct (decide (idx = i)); simplify_map_eq.
-    - rewrite insert_insert_eq.
-      rewrite kvs_keys_insert_None; auto.
-      destruct x as [ [] |].
-      + rewrite kvs_keys_insert_Some in Hnodup; auto.
-        apply NoDup_cons in Hnodup as [ _ Hnodup ]; auto.
-      + rewrite kvs_keys_insert_None in Hnodup; auto.
-    - rewrite insert_insert_ne; auto.
-      destruct x as [ [ k' w' ] |].
-      + rewrite kvs_keys_insert_Some in Hnodup; auto.
-        apply NoDup_cons in Hnodup as [ Hk' Hnodup ]; auto.
-        rewrite kvs_keys_insert_Some; simplify_map_eq; auto.
-        apply NoDup_cons; split ; auto.
-        intro Hk. apply elem_of_kvs_keys in Hk as (?&idx_k&?); simplify_eq.
-        destruct (decide (idx_k = idx)); simplify_map_eq.
-        apply Hk'.
-        apply elem_of_kvs_keys; eexists _,_ ; eauto.
-      + rewrite kvs_keys_insert_None in Hnodup; auto.
-        rewrite kvs_keys_insert_None; simplify_map_eq; auto.
-  Qed.
-
-  Lemma wf_kvs_physical_map_delete (m : kvs_physical_map) (idx : nat) (k : Z) :
-    (is_Some (m !! idx)) ->
-    wf_kvs_physical_map m ->
-    wf_kvs_physical_map (<[idx:=None]> m).
-  Proof.
-    intros [w' Hidx] (Hkvs_dom & Hkvs_unique).
-    split.
-    - rewrite dom_insert_L -Hkvs_dom.
-      assert (idx ∈ dom m).
-      { apply elem_of_dom; eauto. }
-      set_solver.
-    - eapply NoDup_kvs_keys_delete; eauto.
-  Qed.
-
-  (* Lemma isKVS_open_delete (a : Addr) (m : kvs_physical_map) (lm : kvs_logical_map) (umap : kvs_user_map) *)
-  (*   (idx : nat) (uk mk : Z) (w : Word) : *)
-  (*   let k := kvs_full_key uk mk in *)
-  (*   is_uint16 mk -> *)
-  (*   isKVS_open a m lm idx -∗ *)
-  (*   uk ↦(KVS_USER) umap -∗ *)
-  (*   k ⤇(KVS)[ idx ] w *)
-  (*   ==∗ *)
-  (*   isKVS_open a (<[idx:=None]> m) (kvs_logical_kvs_delete lm uk mk) idx ∗ *)
-  (*   uk ↦(KVS_USER) (delete mk umap) ∗ *)
-  (*   idx ⤇(KVS) NONE. *)
-  (* Proof. *)
-  (*   intro k. *)
-  (*   iIntros (Hwf_kvs_full_key) *)
-  (*     "(%Hwf_kvs & %Hwf_alloc & Hkvs_auth & Halloc_auth & HKVS) Halloc_frag Hk". *)
-  (*   iDestruct (kvs_logical_kvs_valid with "Halloc_auth Halloc_frag") as "%Hvalid". *)
-  (*   iDestruct (kvs_valid with "Hkvs_auth Hk") as "%Hm_idx". *)
-  (*   iMod (kvs_auth_delete a m idx _ _ with "Hkvs_auth Hk") as "[$ $]". *)
-
-  (*   iMod ( kvs_logical_kvs_update uk lm umap (delete mk umap) with "Halloc_auth Halloc_frag") as "[Halloc_auth Halloc_frag]". *)
-  (*   assert (NoDup (kvs_keys m)) as Hnodup by ( by destruct Hwf_kvs ). *)
-  (*   rewrite /kvs_synced_logical_kvs in Hwf_alloc. *)
-  (*   eapply (wf_kvs_physical_map_delete _ _) in Hwf_kvs; eauto. *)
-  (*   eapply (kvs_synced_logical_kvs_delete _ _ _ _ _ w) in Hwf_alloc; eauto. *)
-  (*   rewrite delete_insert_eq. *)
-  (*   subst k. *)
-  (*   iFrame "∗ %". *)
-  (*   by rewrite /kvs_logical_kvs_delete Hvalid /=. *)
-  (* Qed. *)
-
 End KVS_preamble.
-
-(* Definition kvs_user_map_auth `{kvsG} (uk : Z) (m : kvs_user_map) : iProp Σ := uk ↦(KVS_USER) m. *)
-(* Definition kvs_user_map_frag `{kvsG} (uk mk : Z) ( w : Word ) : iProp Σ := kvs_full_key uk mk ⤇(KVS) w. *)
-
-(* Notation "'◯↪KVS[' uk ']' m" := (kvs_user_map_auth uk m)%I (at level 20) : bi_scope. *)
-(* Notation "mk '↦(KVS)[' uk ']' w" := (kvs_user_map_frag uk mk w)%I (at level 20) : bi_scope. *)
-(* Notation "mk '↦(KVS)[' uk ']' -" := (∃ w, mk ↦(KVS)[ uk ] w)%I (at level 20) : bi_scope. *)
 
 
 Section KVS_preamble_public.
@@ -1597,29 +1232,12 @@ Section KVS_preamble_public.
       logical_kvs_inv KVS_cgp_b ∗
       seal_pred KVS_OTYPE kvs_otype_propC.
 
-  (* Lemma kvs_pointsto_valid *)
-  (*   (a : Addr) (mkvs : kvs_physical_map) (lm : kvs_logical_map) *)
-  (*   (m : kvs_user_map) (uk mk : Z) (w : Word) : *)
-  (*     is_uint16 mk -> *)
-  (*     isKVS a mkvs lm -∗ *)
-  (*     ◯↪KVS[ uk ] m -∗ *)
-  (*     mk ↦(KVS)[uk] w *)
-  (*     -∗ *)
-  (*     ⌜ m !! mk = Some w ⌝. *)
-  (* Proof. *)
-  (*   iIntros (Hwf_key) "(%Hwk_kvs & %Hsynced & Hkvs & Hlkvs & _) Hm Hmk". *)
-  (*   rewrite /kvs_user_map_auth /kvs_user_map_frag. *)
-  (*   iDestruct ( kvs_logical_kvs_valid with "Hlkvs Hm") as "%Huk". *)
-  (*   iDestruct "Hmk" as "[%idx Hmk]". *)
-  (*   iDestruct (kvs_valid with "Hkvs Hmk" ) as "%Hidx". *)
-  (*   specialize (Hsynced (uk,mk) w Hwf_key); cbn in *. *)
-  (*   assert ( kvs_elem_of_kvs mkvs (kvs_full_key uk mk) w ) as H by (eexists;eauto). *)
-  (*   apply Hsynced in H as (?&?&?); simplify_eq. *)
-  (*   done. *)
-  (* Qed. *)
-
 End KVS_preamble_public.
 
 Global Opaque kvs_physical_map_init.
-(* Global Opaque kvs_user_map_auth. *)
-(* Global Opaque kvs_user_map_frag. *)
+
+Notation "<<[ ( uk , mk ) := w ]>> lkvs" :=
+  (kvs_logical_kvs_insert lkvs uk mk w) (at level 10).
+
+Notation "lkvs <∖> ( uk , mk )" :=
+  (kvs_logical_kvs_delete lkvs uk mk) (at level 10).
